share/everparse/tests/lowparse/LowParseExample10.fst
@@ -1,15 +1,95 @@
 module LowParseExample10
 #lang-pulse
-(* Ported from ifthenelse test.
-   Spec parts are in LowParseExample10.Aux.
-   NOTE: Pulse validator for ifthenelse requires a leaf_reader for
-   parse_flbytes 3, which is not yet available in the Pulse combinator library.
-   The spec (parser, serializer) is fully verified. *)
-
 include LowParseExample10.Aux
+open FStar.Tactics.V2
 open Pulse.Lib.Pervasives
+open Pulse.Lib.Slice
+open LowParse.Spec.Base
 
+module SZ = FStar.SizeT
+module R = Pulse.Lib.Reference
+module S = Pulse.Lib.Slice
+module LPS = LowParse.Pulse.Base
+module LPI = LowParse.Pulse.Int
+module LPC = LowParse.Pulse.Combinators
+module PPB = LowParse.PulseParse.Base
+module PPC = LowParse.PulseParse.Combinators
+module PPITE = LowParse.PulseParse.IfThenElse
+module Trade = Pulse.Lib.Trade.Util
+module U8 = FStar.UInt8
+module U16 = FStar.UInt16
+module U32 = FStar.UInt32
 module I32 = FStar.Int32
+
+(* leaf_reader for parse_u8 *)
+
+inline_for_extraction noextract
+let leaf_read_u8 : PPB.leaf_reader parse_u8 =
+  PPB.leaf_reader_of_serialized (LPI.read_u8' ())
+
+(* leaf_reader for msg_type = parse_u8 `nondep_then` parse_u8 `nondep_then` parse_u8
+   Read the three bytes sequentially using peek_trade_gen *)
+
+#push-options "--z3rlimit 32"
+
+inline_for_extraction
+fn leaf_read_msg_type_fn
+  (input: S.slice byte)
+  (#pm: perm)
+  (#v: Ghost.erased msg_type)
+  requires PPB.pts_to_parsed parse_msg_type input #pm v
+  returns res: msg_type
+  ensures PPB.pts_to_parsed parse_msg_type input #pm v ** pure (res == Ghost.reveal v)
+{
+  PPB.pts_to_parsed_elim input;
+  with w . assert (S.pts_to input #pm w);
+  nondep_then_eq (nondep_then parse_u8 parse_u8) parse_u8 w;
+  nondep_then_eq parse_u8 parse_u8 w;
+  parser_kind_prop_equiv parse_u8_kind parse_u8;
+  let mut poff = 0sz;
+  let _ = LPI.validate_u8 input poff;
+  let off1 = !poff;
+  let a = PPB.read_parsed_from_validator_success leaf_read_u8 input 0sz off1;
+  let _ = LPI.validate_u8 input poff;
+  let off2 = !poff;
+  let b = PPB.read_parsed_from_validator_success leaf_read_u8 input off1 off2;
+  let _ = LPI.validate_u8 input poff;
+  let off3 = !poff;
+  let c = PPB.read_parsed_from_validator_success leaf_read_u8 input off2 off3;
+  PPB.pts_to_parsed_intro_injective parse_msg_type input v;
+  Trade.trans (PPB.pts_to_parsed parse_msg_type input #pm v) (S.pts_to input #pm w) (PPB.pts_to_parsed parse_msg_type input #pm v);
+  Trade.elim (PPB.pts_to_parsed parse_msg_type input #pm v) (PPB.pts_to_parsed parse_msg_type input #pm v);
+  ((a, b), c)
+}
+
+inline_for_extraction noextract
+let leaf_read_msg_type : PPB.leaf_reader parse_msg_type = leaf_read_msg_type_fn
+
+#pop-options
+
+(* Pulse validator *)
+
+inline_for_extraction
+let validate_t : LPS.validator parse_t =
+  PPITE.validate_ifthenelse parse_t_param
+    (PPC.validate_nondep_then (PPC.validate_nondep_then LPI.validate_u8 LPI.validate_u8) LPI.validate_u8)
+    leaf_read_msg_type
+    (fun b -> if b then LPI.validate_u32 else LPI.validate_u16)
+    ()
+
+(* Pulse jumper *)
+
+inline_for_extraction
+let jump_msg_type : LPS.jumper parse_msg_type =
+  LPC.jump_nondep_then (LPC.jump_nondep_then LPI.jump_u8 LPI.jump_u8) LPI.jump_u8
+
+inline_for_extraction
+let jump_t : LPS.jumper parse_t =
+  PPITE.jump_ifthenelse parse_t_param
+    jump_msg_type
+    leaf_read_msg_type
+    (fun b -> if b then LPI.jump_u32 else LPI.jump_u16)
+    ()
 
 fn main ()
   requires emp
